feat: improved foundations and cleaned up documentation (#51)

ToMathlib/Control/OptionT.lean
@@ -5,7 +5,7 @@ Released under Apache 2.0 license as described in the file LICENSE.
 Authors: Devon Tuma
 -/
 import ToMathlib.Control.FreeMonad
-import ToMathlib.Control.LawfulFailure
+import ToMathlib.Control.AlternativeMonad
 import ToMathlib.Control.MonadHom
 import ToMathlib.General
 
@@ -20,6 +20,9 @@ namespace OptionT
 variable {m : Type u → Type v}
   {n : Type u → Type w}
   (f : {α : Type u} →  m α → n α) {α β γ : Type u}
+
+@[simp] lemma run_lift {m : Type u → Type v} [Monad m]
+    {α : Type u} (x : m α) : (OptionT.lift x).run = x := rfl
 
 -- @[simp]
 lemma monad_pure_eq_pure [Monad m] (x : α) :
@@ -47,40 +50,42 @@ given an `Alternative n` instance to handle failure. -/
 protected def mapM {m : Type u → Type v} {n : Type u → Type w}
     [AlternativeMonad n] (f : {α : Type u} → m α → n α)
     {α : Type u} (x : OptionT m α) : n α :=
-  do match (← f x.run) with | some x => return x | none => failure
+  do (← f x.run).getM
 
-protected def mapM' {m : Type u → Type v} {n : Type u → Type w}
-    [Monad m] [AlternativeMonad n] [LawfulAlternative n]
-    (f : m →ᵐ n) : OptionT m →ᵐ n where
-  toFun x := do match (← f x.run) with
-    | some x => return x
-    | none => failure
-  toFun_pure' x := by
-    simp
-  toFun_bind' x y := by
-    simp
-    congr 1
-    ext x
-    cases x
-    simp
-    simp
+-- protected def mapM' {m : Type u → Type v} {n : Type u → Type w}
+--     [Monad m] [Monad n] [AlternativeMonad n] [LawfulAlternative n]
+--     (f : m →ᵐ n) : OptionT m →ᵐ n where
+--   toFun x := do match (← f x.run) with
+--     | some x => return x
+--     | none => failure
+--   toFun_pure' x := by
+--     simp
+--     rw [pure_bind]
+--   toFun_bind' x y := by
+--     simp
+--     congr 1
+--     ext x
+--     cases x
+--     simp
+--     simp
 
-@[simp]
-lemma mapM'_lift {m : Type u → Type v} {n : Type u → Type w}
-    [Monad m] [AlternativeMonad n] [LawfulAlternative n]
-    (f : m →ᵐ n) (x : m α) : OptionT.mapM' f (OptionT.lift x) = f x := by
-  simp [OptionT.mapM', OptionT.lift]
+-- @[simp]
+-- lemma mapM'_lift {m : Type u → Type v} {n : Type u → Type w}
+--     [Monad m] [AlternativeMonad n] [LawfulAlternative n]
+--     (f : m →ᵐ n) (x : m α) : OptionT.mapM' f (OptionT.lift x) = f x := by
+--   simp [OptionT.mapM', OptionT.lift]
 
-@[simp]
-lemma mapM'_failure {m : Type u → Type v} {n : Type u → Type w}
-    [Monad m] [AlternativeMonad n] [LawfulAlternative n]
-    (f : m →ᵐ n) : OptionT.mapM' f (failure : OptionT m α) = failure := by
-  simp [OptionT.mapM']
+-- @[simp]
+-- lemma mapM'_failure {m : Type u → Type v} {n : Type u → Type w}
+--     [Monad m] [AlternativeMonad n] [LawfulAlternative n]
+--     (f : m →ᵐ n) : OptionT.mapM' f (failure : OptionT m α) = failure := by
+--   simp [OptionT.mapM']
 
-lemma mapM_pure [Monad m] [AlternativeMonad n] [LawfulAlternative n]
-    (h : ∀ {α} (x : α), f (OptionT.pure x).run = pure x) (x : α) :
-    OptionT.mapM f (pure x : OptionT m α) = pure x := by
-  simp [OptionT.mapM, h, OptionT.monad_pure_eq_pure]
+-- lemma mapM_pure [Monad m] [Monad n] [LawfulMonad n] [AlternativeMonad n] [LawfulAlternative n]
+--     (h : ∀ {α} (x : α), f (OptionT.pure x).run = pure x) (x : α) :
+--     OptionT.mapM f (pure x : OptionT m α) = pure x := by
+--   simp [OptionT.mapM, h, OptionT.monad_pure_eq_pure]
+
 
 end mapM
 
