VCVio/CryptoFoundations/AsymmEncAlg.lean
@@ -6,6 +6,7 @@ Authors: Devon Tuma
 import VCVio.CryptoFoundations.SecExp
 import VCVio.OracleComp.Constructions.UniformSelect
 import VCVio.OracleComp.Coercions.SubSpec
+import VCVio.OracleComp.SimSemantics.Append
 
 /-!
 # Asymmetric Encryption Schemes.
@@ -15,115 +16,158 @@ for asymmetric encryption using oracles in `spec`, with message space `M`,
 public/secret keys `PK` and `SK`, and ciphertext space `C`.
 -/
 
-open OracleSpec OracleComp
+open OracleSpec OracleComp ENNReal
 
 universe u v w
 
-structure AsymmEncAlg {ι : Type} (spec : OracleSpec ι) (em : Type → Type v)
-    (M PK SK C : Type) extends ExecutionMethod spec em where
-  keygen : OracleComp spec (PK × SK)
-  encrypt (m : M) (pk : PK) : OracleComp spec C
-  decrypt (c : C) (sk : SK) : OracleComp spec M
+/-- An `AsymmEncAlg` with message space `M`, key spaces `PK` and `SK`, and ciphertexts in `C`.
+`spec` is the available oracle set and `m` is the monad used to execute the oracle calls.
+Extends `ExecutionMethod spec m`, in most cases will be `ExecutionMethod.default`. -/
+structure AsymmEncAlg (m : Type → Type u) (M PK SK C : Type)
+    extends ExecutionMethod m where
+  keygen : m (PK × SK)
+  encrypt : (pk : PK) → (msg : M) →  m C
+  decrypt : (sk : SK) → (c : C) → Option M
+
+alias PKE_Alg := AsymmEncAlg
 
 namespace AsymmEncAlg
 
-variable {ι : Type} {spec : OracleSpec ι} {M PK SK C : Type}
-    {em : Type → Type v} [AlternativeMonad em] [LawfulAlternative em]
+variable {ι : Type} {spec : OracleSpec ι} {m : Type → Type v} {M PK SK C : Type}
+  (encAlg : AsymmEncAlg m M PK SK C) {α β γ : Type}
 
-section sound
+section Correct
 
--- variable [Π sp, DecidableEq (M sp)]
+-- variable [AlternativeMonad m] [LawfulAlternative m] [DecidableEq M]
+variable [DecidableEq M] [AlternativeMonad m]
 
+/-- A `SymmEncAlg` is complete if decrypting an encrypted message always returns that original
+message, captured here by a `guard` statement. -/
+@[reducible, inline]
+-- def CorrectExp (encAlg : AsymmEncAlg spec m M PK SK C) (msg : M) :
+--     ProbComp Unit := encAlg.exec do
+--   let (pk, sk) ← encAlg.keygen
+--   guard (encAlg.decrypt sk (← encAlg.encrypt pk msg) = msg)
 
--- /-- Experiment for checking that an asymmetric encryption algorithm is sound,
--- i.e. that decryption properly reverses encryption -/
--- def soundnessExp (encAlg : AsymmEncAlg spec M PK SK C)
---     (mDist : (sp : ℕ) → OracleComp (spec sp) (M sp)) :
---     SecExp spec where
---   main := λ sp ↦ do
---     let m ← mDist sp
---     let (pk, sk) ← encAlg.keygen sp
---     let σ ← encAlg.encrypt sp m pk
---     let m' ← encAlg.decrypt sp σ sk
---     return m = m'
---   __ := encAlg
+def CorrectExp (encAlg : AsymmEncAlg m M PK SK C) (msg : M) :
+    ProbComp Unit := encAlg.exec do
+  let (pk, sk) ← encAlg.keygen
+  guard (encAlg.decrypt sk (← encAlg.encrypt pk msg) = msg)
 
-def soundnessExp [DecidableEq M] (encAlg : AsymmEncAlg spec em M PK SK C)
-    (m : M) : SecExp spec em where
-  main := do
+/-- Perfectly correct if messages never fail to decrypt back to themselves for any message. -/
+-- def PerfectlyCorrect (encAlg : AsymmEncAlg spec m M PK SK C) : Prop :=
+--   ∀ (msg : M), [⊥ | CorrectExp encAlg msg] = 0
+
+def PerfectlyCorrect (encAlg : AsymmEncAlg m M PK SK C) : Prop :=
+  ∀ (msg : M), [⊥ | CorrectExp encAlg msg] = 0
+
+-- @[simp] lemma PerfectlyCorrect_iff : encAlg.PerfectlyCorrect ↔
+--     ∀ (msg : M), [⊥ | CorrectExp encAlg msg] = 0 := Iff.rfl
+
+@[simp] lemma PerfectlyCorrect_iff (encAlg : AsymmEncAlg m M PK SK C) :
+    PerfectlyCorrect encAlg ↔
+    ∀ (msg : M), [⊥ | CorrectExp encAlg msg] = 0 := Iff.rfl
+
+end Correct
+
+section decryptionOracle
+
+variable [AlternativeMonad m]
+
+/-- Oracle that uses a secret key to respond to decryption requests. -/
+def decryptionOracle (encAlg : AsymmEncAlg m M PK SK C)
+    (sk : SK) : QueryImpl (C →ₒ M) m where
+  impl | query () c => Option.getM (encAlg.decrypt sk c)
+
+@[simp]
+lemma decryptionOracle.apply_eq (encAlg : AsymmEncAlg m M PK SK C)
+    (sk : SK) (q : OracleQuery (C →ₒ M) α) : (decryptionOracle encAlg sk).impl q =
+    match q with | query () c => Option.getM (encAlg.decrypt sk c) := rfl
+
+end decryptionOracle
+
+section IND_CCA
+
+variable [AlternativeMonad m] [LawfulAlternative m] [DecidableEq C]
+
+/-- Two oracles for IND-CCA Experiment, the first for decrypting ciphertexts, and the second
+for getting a challenge from a pair of messages. -/
+def IND_CCA_oracleSpec (_encAlg : AsymmEncAlg m M PK SK C) :=
+    (C →ₒ Option M) ++ₒ ((M × M) →ₒ C)
+
+/-- Implement oracles for IND-CCA security game. A state monad is to track the current challenge,
+if it exists, and is set by the adversary calling the second oracle.
+The decryption oracle checks to make sure it doesn't decrypt the challenge. -/
+def IND_CCA_oracleImpl [DecidableEq C] (encAlg : AsymmEncAlg m M PK SK C)
+    (pk : PK) (sk : SK) (b : Bool) : QueryImpl (IND_CCA_oracleSpec encAlg)
+      (StateT (Option C) m) where impl
+  | query (Sum.inl ()) c => do
+      guard ((← get) ≠ some c)
+      return encAlg.decrypt sk c
+  | query (Sum.inr ()) (m₁, m₂) => do
+      guard (← get).isNone
+      let c ← encAlg.encrypt pk (if b then m₁ else m₂)
+      set (some c)
+      return c
+
+structure IND_CCA_Adversary (encAlg : AsymmEncAlg m M PK SK C) where
+    main : PK → OracleComp encAlg.IND_CCA_oracleSpec Bool
+
+def IND_CCA_Game (encAlg : AsymmEncAlg m M PK SK C)
+    (adversary : encAlg.IND_CCA_Adversary) : ProbComp Unit :=
+  encAlg.exec do
     let (pk, sk) ← encAlg.keygen
-    let σ ← encAlg.encrypt m pk
-    let m' ← encAlg.decrypt σ sk
-    guard (m' = m)
-  __ := encAlg
-
--- def IsSound [DecidableEq M] (encAlg : AsymmEncAlg spec em M PK SK C) : Prop :=
---   ∀ m : M, (soundnessExp encAlg m).advantage = 1
-
-def IsSound [DecidableEq M] (encAlg : AsymmEncAlg spec em M PK SK C) : Prop :=
-    ∀ m : M, [⊥ | encAlg.exec do
-      let (pk, sk) ← encAlg.keygen
-      let σ ← encAlg.encrypt m pk
-      let m' ← encAlg.decrypt σ sk
-      guard (m' = m)] = 0
-
-
--- namespace soundnessExp
-
-
--- end soundnessExp
-
--- /-- An asymmetric encryption algorithm is sound if messages always decrypt to themselves. -/
--- def isSound (encAlg : AsymmEncAlg spec M PK SK C) : Prop :=
---   ∀ mDist, negligible (1 - (soundnessExp encAlg mDist).advantage)
-
--- -- lemma sound_iff [DecidableEq M] (encAlg : AsymmEncAlg spec M PK SK C) : encAlg.isSound ↔
--- --     ∀ m : M, ∀ m' ∈ (encAlg.exec <| do
--- --       let (pk, sk) ← encAlg.keygen ()
--- --       let σ ← encAlg.encrypt m pk
--- --       encAlg.decrypt σ sk).support, m = m' := by
--- --   simp only [isSound, SecExp.advantage_eq_one_iff]
--- --   sorry
-
-end sound
-
-section IND_CPA
-
--- variable [DecidableEq ι]
-
-variable [DecidableEq ι]
-
-/-- `IND_CPA_adv M PK C` is an adversary for IND-CPA security game on an
-asymmetric encryption with public keys in `PK`, messages in `M`, and ciphertexts in `C`.
-Adversary is given a public key and returns a pair of messages that it thinks
-it can distinguish the encryption of. It addionally has a `distinguish` function
-that given a pair of messages and an encryption, returns whether it is an encryption of
-the first message or the second message.
-TODO: should use sim oracles to allow state sharing -/
-structure IND_CPA_Adv (encAlg : AsymmEncAlg spec em M PK SK C)
-    extends SecAdv spec PK (M × M) where
-  distinguish : PK → M × M → C → OracleComp spec Bool
-
-/-- Experiment for IND-CPA security of an asymmetric encryption algorithm.
-`inp_gen` generates a key and pre-selects a random boolean value.
-`main` runs the adversary on the public key, and encrypts the resulting message corresponding to
-the boolean chosen in `inp_gen`, finally asking the adversary to determine the boolean
-given the messages and resulting ciphertext. `is_valid` checks that this choice is correct.
-The simulation oracles are pulled in directly from the encryption algorithm. -/
-def IND_CPA_Exp [unifSpec ⊂ₒ spec]
-    {encAlg : AsymmEncAlg spec em M PK SK C}
-    (adv : IND_CPA_Adv encAlg) :
-    SecExp spec em where
-  main := do
-    let (pk, _) ← encAlg.keygen
-    let (m₁, m₂) ← adv.run pk
-    let b : Bool ←$ᵗ Bool
-    let m := if b then m₁ else m₂
-    let c ← encAlg.encrypt m pk
-    let b' ← adv.distinguish pk (m₁, m₂) c
+    let b ← encAlg.lift_probComp ($ᵗ Bool)
+    let b' ← (simulateQ (encAlg.IND_CCA_oracleImpl pk sk b) (adversary.main pk)).run' none
     guard (b = b')
-  __ := encAlg
 
-end IND_CPA
+end IND_CCA
+
+-- section IND_CPA
+
+-- -- variable [DecidableEq ι]
+
+-- variable [AlternativeMonad m] [LawfulAlternative m] [DecidableEq ι]
+
+-- /-- `IND_CPA_adv M PK C` is an adversary for IND-CPA security game on an
+-- asymmetric encryption with public keys in `PK`, messages in `M`, and ciphertexts in `C`.
+-- Adversary is given a public key and returns a pair of messages that it thinks
+-- it can distinguish the encryption of. It addionally has a `distinguish` function
+-- that given a pair of messages and an encryption, returns whether it is an encryption of
+-- the first message or the second message.
+-- TODO: should use sim oracles to allow state sharing -/
+-- structure IND_CPA_Adv (encAlg : AsymmEncAlg m M PK SK C)
+--     extends SecAdv spec PK (M × M) where
+--   distinguish : PK → M × M → C → OracleComp spec Bool
+
+-- /-- Experiment for IND-CPA security of an asymmetric encryption algorithm.
+-- `inp_gen` generates a key and pre-selects a random boolean value.
+-- `main` runs the adversary on the public key, and encrypts the resulting message corresponding to
+-- the boolean chosen in `inp_gen`, finally asking the adversary to determine the boolean
+-- given the messages and resulting ciphertext. `is_valid` checks that this choice is correct.
+-- The simulation oracles are pulled in directly from the encryption algorithm. -/
+-- def IND_CPA_Exp [unifSpec ⊂ₒ spec]
+--     {encAlg : AsymmEncAlg m M PK SK C}
+--     (adv : IND_CPA_Adv encAlg) : ProbComp Unit :=
+--   encAlg.exec do
+--     let (pk, _) ← encAlg.keygen
+--     let (m₁, m₂) ← adv.run pk
+--     let b : Bool ←$ᵗ Bool
+--     let m := if b then m₁ else m₂
+--     let c ← encAlg.encrypt pk m
+--     let b' ← adv.distinguish pk (m₁, m₂) c
+--     guard (b = b')
+
+--   -- main := do
+--   --   let (pk, _) ← encAlg.keygen
+--   --   let (m₁, m₂) ← adv.run pk
+--   --   let b : Bool ←$ᵗ Bool
+--   --   let m := if b then m₁ else m₂
+--   --   let c ← encAlg.encrypt pk m
+--   --   let b' ← adv.distinguish pk (m₁, m₂) c
+--   --   guard (b = b')
+--   -- __ := encAlg
+
+-- end IND_CPA
 
 end AsymmEncAlg
