ToMathlib/Control/Lawful/MonadState.lean
@@ -13,6 +13,12 @@ This file defines the `LawfulMonadState(Of)` class, which adds laws to the `Mona
 
 universe u v w
 
+@[simp] theorem toMonadState_get_eq_monadStateOf_get {m : Type u → Type v} {σ : Type u}
+    [MonadStateOf σ m] : (MonadState.get : m σ) = MonadStateOf.get := rfl
+
+@[simp] theorem toMonadState_set_eq_monadStateOf_set {m : Type u → Type v} {σ : Type u}
+    [MonadStateOf σ m] : (MonadState.set : σ → m PUnit) = MonadStateOf.set := rfl
+
 class LawfulMonadStateOf (σ : outParam (Type u)) (m : Type u → Type v) [Monad m] [MonadStateOf σ m]
     : Prop where
 
@@ -21,9 +27,11 @@ class LawfulMonadStateOf (σ : outParam (Type u)) (m : Type u → Type v) [Monad
     MonadStateOf.modifyGet (m := m) f = do let (a, s) := f (← MonadStateOf.get); set s; pure a
 
   /-- `get` twice doesn't change the state -/
-  get_get : {α : Type u} → {a : σ → σ → m α} →
-    (do let s₁ ← MonadStateOf.get; let s₂ ← MonadStateOf.get; a s₁ s₂)
-      = do let s ← MonadStateOf.get; a s s
+  get_get : (MonadStateOf.get : m σ) *> (MonadStateOf.get : m σ) = MonadStateOf.get
+
+  -- {a : σ → σ → m α} →
+  --   (do let s₁ ← MonadStateOf.get; let s₂ ← MonadStateOf.get; a s₁ s₂)
+  --     = do let s ← MonadStateOf.get; a s s
 
   /-- `set` twice has the same effect as the second `set` -/
   set_set : {s₁ s₂ : σ} → (do set s₁; set s₂) = set (m := m) s₂
@@ -60,16 +68,16 @@ theorem modifyThe_eq (f : σ → σ) :
 
 end LawfulMonadStateOf
 
-class LawfulMonadState (σ : outParam (Type u)) (m : Type u → Type v) [Monad m]
-    extends MonadState σ m : Type (max (u+1) v) where
+-- TOOD: don't think this should extend, same way `LawfulMonad` doesn't.
+class LawfulMonadState (σ : outParam (Type u)) (m : Type u → Type v) [Monad m] :
+    Type (max (u+1) v) extends MonadState σ m where
 
   /-- `modifyGet f` is equivalent to `do let (a, s) := f (← get); set s; pure a` -/
   modifyGet_eq : {α : Type u} → (f : σ → α × σ) →
     modifyGet f = do let (a, s) := f (← get); set s; pure a
 
   /-- `get` twice doesn't change the state -/
-  get_get : {α : Type u} → {a : σ → σ → m α} →
-    (do let s₁ ← get; let s₂ ← get; a s₁ s₂) = (do let s ← get; a s s)
+  get_get : get *> get = get
 
   /-- `set` twice has the same effect as the second `set` -/
   set_set : {s₁ s₂ : σ} → (do set s₁; set s₂) = set s₂
@@ -93,10 +101,14 @@ theorem modify_eq (f : σ → σ) :
   simp only [modify, modifyGet_eq, bind_pure_comp, id_map']
 
 -- Do we need extra property of `get` here? That `get` twice is the same as `get` once?
-@[simp]
-theorem getModify_eq (f : σ → σ) :
-    getModify (m := m) f = get <* modify f := by
-  simp [getModify, seqLeft_eq_bind]
+-- @[simp]
+-- theorem getModify_eq (f : σ → σ) :
+--     getModify (m := m) f = get <* modify f := by
+--   simp [getModify, seqLeft_eq_bind]
+--   refine bind_congr fun s => ?_
+--   sorry
+  -- have := bind_assoc get
+  -- rw [← bind_assoc get get]
 
 end LawfulMonadState
 
@@ -107,6 +119,23 @@ instance {σ : Type u} {m : Type u → Type v} [Monad m] [LawfulMonad m] [MonadS
   set_set := LawfulMonadStateOf.set_set
   get_set := LawfulMonadStateOf.get_set
   set_get := LawfulMonadStateOf.set_get
+
+-- instance  {m : Type u → Type v} {n : Type u → Type w} {σ : Type u}
+--     [Monad m] [Monad n] [MonadLift m n] [MonadStateOf σ m]
+--     [LawfulMonad m] [LawfulMonad n] [LawfulMonadLift m n] [LawfulMonadStateOf σ m] :
+--       LawfulMonadStateOf σ n where
+--   modifyGet_eq f := by
+--     simp [MonadStateOf.modifyGet, LawfulMonadState.modifyGet_eq, bind_pure_comp,
+--       MonadStateOf.get, liftM, MonadStateOf.set]
+--   get_get {α} {f} := by {
+--     simp [MonadStateOf.get]
+--     rw [bind_assoc]
+--     rw [← LawfulMonadStateOf.get_get (m := m)]
+--     sorry
+--   }
+--   set_set := sorry
+--   get_set := sorry
+--   set_get := sorry
 
 namespace StateT
 
@@ -138,8 +167,18 @@ instance : LawfulMonadStateOf σ (StateT σ m) where
   modifyGet_eq f := by
     simp only [MonadStateOf.modifyGet, modifyGet_eq_monadState, pure, MonadStateOf.get, set]
   get_get := by
-    intro α a
-    simp only [MonadStateOf.get, get_get]
+    -- intro α a
+    simp only [MonadStateOf.get, get_get, StateT.get]
+    unfold StateT.get
+    simp [seqRight_eq]
+    simp [seq_eq_bind]
+    refine funext fun s => ?_
+    show _ >>= _ = _
+    simp
+    -- rw [StateT.run_bind]
+    -- apply StateT.ext fun s => ?_
+    -- rw [StateT.run_bind]
+    -- simp [StateT.run]
   set_set := by
     intro s₁ s₂
     simp only [set, set_set]
@@ -148,21 +187,6 @@ instance : LawfulMonadStateOf σ (StateT σ m) where
     simp only [set, MonadStateOf.get, get_set, pure]
   set_get := by
     simp only [MonadStateOf.get, set, set_get, pure]
-
 instance : LawfulMonadState σ (StateT σ m) := inferInstance
-
--- TODO: finish proof
-instance {n : Type u → Type w} [Monad m] [Monad n] [MonadLift m n] [MonadStateOf σ m]
-    [LawfulMonad m] [LawfulMonad n] [LawfulMonadLift m n] [LawfulMonadStateOf σ m] :
-      LawfulMonadStateOf σ n where
-  modifyGet_eq f := by
-    simp only [MonadStateOf.modifyGet, LawfulMonadState.modifyGet_eq, bind_pure_comp,
-      MonadStateOf.get, liftM, set]
-    sorry
-
-  get_get := sorry
-  set_set := sorry
-  get_set := sorry
-  set_get := sorry
 
 end StateT
