VCVio/CryptoFoundations/FiatShamir.lean
@@ -5,7 +5,7 @@ Authors: Devon Tuma
 -/
 import VCVio.CryptoFoundations.SigmaAlg
 import VCVio.CryptoFoundations.SignatureAlg
-import VCVio.OracleComp.SimSemantics.QueryTracking.RandOracle
+import VCVio.OracleComp.QueryTracking.CachingOracle
 import VCVio.OracleComp.Coercions.Append
 
 /-!
@@ -14,6 +14,8 @@ import VCVio.OracleComp.Coercions.Append
 This file defines a basic version of the Fiat-Shamir transform on sigma protocols.
 For simplicity we construct signature schemes rather than general proofs of knowledge.
 -/
+
+universe u v
 
 -- TODO
 open OracleComp OracleSpec
@@ -27,8 +29,12 @@ open OracleComp OracleSpec
 --     [Π n, Fintype (X n)] [Π n, Inhabited (X n)] [Π n, SelectableType (X n)]
 --     [Π n, Fintype (W n)] [Π n, Inhabited (W n)] [Π n, SelectableType (W n)]
 
-variable {ι : Type} {spec : OracleSpec ι} {σ X W : Type}
-    {p : X → W → Bool} {PC SC Ω P : Type}
+
+section genrel
+
+variable {ι : Type} {spec : OracleSpec ι} {m : Type → Type v} {σ X W : Type}
+    {p : X → W → Bool} {PC SC Ω P : Type} [Monad m]
+    [SelectableType X] [SelectableType W] (M : Type)
 
 
 -- /-- Given a Σ-protocol we get a signature algorithm by using a random oracle to generate
@@ -37,29 +43,40 @@ variable {ι : Type} {spec : OracleSpec ι} {σ X W : Type}
 --     (M : Type) :
 --     SignatureAlg spec σ M X W (PC × P) := sorry
 
--- def FiatShamir (sigmaAlg : SigmaAlg (λ n ↦ spec n) X W p PC SC Ω P)
---     (hr : GenerableRelation spec X W p) :
---     SignatureAlg (λ n ↦ spec n ++ₒ (M n × PC n →ₒ Ω n))
---       (M := M) (PK := X) (SK := W)
---       (S := λ n ↦ PC n × P n) where
---   -- Use the existing algorithm for generating relation members
---   keygen := λ n ↦ hr.gen n
---   -- Sign by running the sigma protocol using a hash as the challenge
---   sign := λ n pk sk m ↦ do
---     let (c, e) ← sigmaAlg.commit n pk sk
---     let r ← query (Sum.inr <| Sum.inr ()) (m, c)
---     let s ← sigmaAlg.respond n pk sk e r
---     return (c, s)
---   -- Verify a signature by checking the challenge returned by the random oracle
---   verify := λ n pk m (c, s) ↦ do
---     let r' ← query (Sum.inr <| Sum.inr ()) (m, c)
---     return sigmaAlg.verify n pk c r' s
---   -- Simulation includes an additional cache for random oracle
---   baseState := λ n ↦ sigmaAlg.baseState n × QueryCache _
---   -- Add an empty cache to initial state
---   init_state := λ n ↦ (sigmaAlg.init_state n, ∅)
---   -- Simulate the additional oracle as a random oracle
---   baseSimOracle := λ n ↦ sigmaAlg.baseSimOracle n ++ₛₒ randOracle
+structure GenerableRelation
+    (X W : Type) (r : X → W → Bool)
+    [SelectableType X] [SelectableType W] where
+  gen : ProbComp (X × W)
+  gen_sound (x : X) (w : W) : (x, w) ∈ gen.support → r x w
+  gen_uniform_right (x : X) : [= x | Prod.fst <$> gen] = [= x | $ᵗ X]
+  gen_uniform_left (w : W) : [= w | Prod.snd <$> gen] = [= w | $ᵗ W]
+
+end genrel
+
+variable {ι : Type} {spec : OracleSpec ι} {σ X W PC SC Ω P : Type}
+    {p : X → W → Bool} [SelectableType X] [SelectableType W]
+    [DecidableEq PC] [DecidableEq Ω] [SelectableType Ω]
+
+def FiatShamir (sigmaAlg : SigmaAlg X W PC SC Ω P p)
+    (hr : GenerableRelation X W p) (M : Type) [DecidableEq M] :
+    SignatureAlg (OracleComp (unifSpec ++ₒ (M × PC →ₒ Ω)))
+      (M := M) (PK := X) (SK := W) (S := PC × P) where
+  keygen := hr.gen
+  sign := fun pk sk m => do
+    let (c, e) ← sigmaAlg.commit pk sk
+    let r ← query (spec := (M × PC →ₒ Ω)) () (m, c)
+    let s ← sigmaAlg.respond pk sk e r
+    return (c, s)
+  verify := fun pk m (c, s) => do
+    let r' ← query (spec := (M × PC →ₒ Ω)) () (m, c)
+    return sigmaAlg.verify pk c r' s
+  exec comp :=
+    let so : QueryImpl (unifSpec ++ₒ (M × PC →ₒ Ω))
+      (StateT ((M × PC →ₒ Ω).QueryCache) ProbComp) :=
+      idOracle ++ₛₒ randomOracle
+    StateT.run' (simulateQ so comp) ∅
+  lift_probComp := monadLift
+  exec_lift_probComp c := by sorry --simp
 
 namespace FiatShamir
 
