VCVio/CryptoFoundations/KeyEncapMech.lean
@@ -1,0 +1,16 @@
+/-
+Copyright (c) 2025 Devon Tuma. All rights reserved.
+Released under Apache 2.0 license as described in the file LICENSE.
+Authors: Devon Tuma
+-/
+import VCVio.CryptoFoundations.SecExp
+import VCVio.OracleComp.Constructions.UniformSelect
+import VCVio.OracleComp.Coercions.SubSpec
+import VCVio.OracleComp.SimSemantics.Append
+
+/-!
+# Key Encapsulation Mechanisms
+
+This file defines a type to represent protocols for key encapsulation mechanisms.
+We also define basic correctness and security properties for these protocols.
+-/
