VCVio/OracleComp/DistSemantics/Simulate.lean
@@ -10,6 +10,8 @@ import ToMathlib.Control.WriterT
 # Lemmas About the Distribution Semantics of `simulateQ`
 
 This file collects various lemmas about the output distributions of `simulateQ`
+
+TODO: probably put these in simulate folder as about the query impl itself
 -/
 
 
@@ -21,22 +23,25 @@ namespace OracleComp
 
 variable {ι : Type u} {spec : OracleSpec ι} {α β γ : Type u} [hs : spec.FiniteRange]
 
-/-- If `fst <$> so i (t, s)` has the same distribution as `query i t` for any state `s`,
-Then `simulate' so` doesn't change the output distribution.
-Stateless oracles are the most common example of this
-TODO: move-/
-lemma evalDist_simulate'_eq_evalDist {σ α : Type u} (so : QueryImpl spec (StateT σ (OracleComp spec)))
-    (h : ∀ i t s, (evalDist ((so.impl (query i t)).run' s)) =
-      OptionT.lift (PMF.uniformOfFintype (spec.range i)))
-    (s : σ) (oa : OracleComp spec α) : evalDist (simulate' so s oa) = evalDist oa := by
-  revert s
-  induction oa using OracleComp.inductionOn with
-  | pure x => simp
-  | query_bind i t oa hoa => exact (λ s ↦ by
-      simp only [StateT.run'_eq] at h
-      simp only [simulate'_bind, simulate_query, evalDist_bind, Function.comp_def, hoa,
-        evalDist_query, ← h i t s, evalDist_map, PMF.bind_map, hoa, bind_map_left])
-  | failure => intro s; rw [simulate'_failure]
+-- /-- If `fst <$> so i (t, s)` has the same distribution as `query i t` for any state `s`,
+-- Then `simulate' so` doesn't change the output distribution.
+-- Stateless oracles are the most common example of this
+-- TODO: move-/
+-- lemma evalDist_simulate'_eq_evalDist {σ α : Type u}
+--     (so : QueryImpl spec (StateT σ (OracleComp spec)))
+--     (h : ∀ i t s, (evalDist ((so.impl (query i t)).run' s)) =
+--       OptionT.lift (PMF.uniformOfFintype (spec.range i)))
+--     (s : σ) (oa : OracleComp spec α) : evalDist ((simulateQ so oa).run' s) = evalDist oa := by
+--   revert s
+--   induction oa using OracleComp.inductionOn with
+--   | pure x => simp
+--   | query_bind i t oa hoa => exact (λ s ↦ by
+--       simp only [StateT.run'_eq] at h
+--       simp [← h i t s, Function.comp_def]
+
+--       sorry
+--       )
+--   | failure => intro s; simp
 
 -- lemma probFailure_simulateQ_WriterT_eq_probFailure {ω : Type u} [Monoid ω]
 --     (so : QueryImpl spec (WriterT ω (OracleComp spec)))
