VCVio/OracleComp/NoFailure.lean
@@ -1,196 +1,189 @@
-/-
-Copyright (c) 2025 Devon Tuma. All rights reserved.
-Released under Apache 2.0 license as described in the file LICENSE.
-Authors: Devon Tuma, Quang Dao
--/
-import VCVio.OracleComp.DistSemantics.Support
+-- /-
+-- Copyright (c) 2025 Devon Tuma. All rights reserved.
+-- Released under Apache 2.0 license as described in the file LICENSE.
+-- Authors: Devon Tuma, Quang Dao
+-- -/
+-- import VCVio.OracleComp.Support
 
-/-!
-# Computations that Never Fail
+-- /-!
+-- # Computations that Never Fail
 
-This file defines a class `OracleComp.NoFailure` for computations that never fail regardless
-of the behavior of oracles. This can be useful for simplifying some probability calculations.
--/
+-- This file defines a class `OracleComp.NoFailure` for computations that never fail regardless
+-- of the behavior of oracles. This can be useful for simplifying some probability calculations.
+-- -/
 
-universe u v w
+-- universe u v w
 
-open OracleSpec
+-- open OracleSpec
 
-namespace OracleComp
+-- namespace OracleComp
 
-variable {ι : Type*} {spec : OracleSpec ι}
+-- variable {ι : Type*} {spec : OracleSpec ι}
 
-def noFailure {α : Type u} (oa : OracleComp spec α) : Prop := by
-  induction oa using OracleComp.construct with
-  | pure _ => exact True
-  | failure => exact False
-  | query_bind _ _ r => exact ∀ x, r x
+-- -- TODO: @[deprecated "OracleComp.neverFailsWhen" (since := "")]
+-- def noFailure {α : Type u} (oa : OracleComp spec α) : Prop := by
+--   induction oa using OracleComp.construct with
+--   | pure _ => exact True
+--   | failure => exact False
+--   | query_bind _ _ r => exact ∀ x, r x
 
-variable {α β γ : Type u}
+-- variable {α β γ : Type u}
 
-lemma noFailure_eq_oracleComp_construct (oa : OracleComp spec α) :
-    oa.noFailure = OracleComp.construct
-      (fun _ ↦ True) (fun {β} _ _ r ↦ ∀ (x : β), r x) False oa := rfl
+-- lemma noFailure_eq_oracleComp_construct (oa : OracleComp spec α) :
+--     oa.noFailure = OracleComp.construct
+--       (fun _ ↦ True) (fun {β} _ _ r ↦ ∀ (x : β), r x) False oa := rfl
 
-lemma noFailure_eq_freeMonad_construct (oa : OracleComp spec α) :
-    oa.noFailure = FreeMonad.construct
-      (fun t ↦ Option.rec False (fun _ ↦ True) t) (fun _ _ r ↦ ∀ x, r x) oa := rfl
+-- lemma noFailure_eq_freeMonad_construct (oa : OracleComp spec α) :
+--     oa.noFailure = FreeMonad.construct
+--       (fun t ↦ Option.rec False (fun _ ↦ True) t) (fun _ _ r ↦ ∀ x, r x) oa := rfl
 
-@[simp]
-lemma noFailure_pure (x : α) : noFailure (pure x : OracleComp spec α) := trivial
+-- @[simp]
+-- lemma noFailure_pure (x : α) : noFailure (pure x : OracleComp spec α) := trivial
 
-@[simp]
-lemma noFailure_query (q : OracleQuery spec α) : noFailure (q : OracleComp spec α) :=
-  fun _ => trivial
+-- @[simp]
+-- lemma noFailure_query (q : OracleQuery spec α) : noFailure (q : OracleComp spec α) :=
+--   fun _ => trivial
 
-@[simp]
-lemma noFailure_query_bind_iff {q : OracleQuery spec α} {oa : α → OracleComp spec β} :
-    (liftM q >>= oa).noFailure ↔ ∀ x, noFailure (oa x) := by
-  simp [liftM, monadLift, MonadLift.monadLift, lift, OptionT.lift, OptionT.mk, bind, OptionT.bind]
-  rw [noFailure_eq_freeMonad_construct]
-  unfold FreeMonad.construct
-  exact Eq.to_iff (by simp_rw [noFailure_eq_freeMonad_construct])
+-- @[simp]
+-- lemma noFailure_query_bind_iff {q : OracleQuery spec α} {oa : α → OracleComp spec β} :
+--     (liftM q >>= oa).noFailure ↔ ∀ x, noFailure (oa x) := Iff.rfl
 
-alias ⟨noFailure_query_bind, _⟩ := noFailure_query_bind_iff
+-- alias ⟨noFailure_query_bind, _⟩ := noFailure_query_bind_iff
 
-@[simp]
-lemma not_noFailure_failure : ¬ noFailure (failure : OracleComp spec α) := fun h => h
+-- @[simp]
+-- lemma not_noFailure_failure : ¬ noFailure (failure : OracleComp spec α) := fun h => h
 
-@[simp]
-lemma noFailure_bind_iff (oa : OracleComp spec α) (ob : α → OracleComp spec β) :
-    (oa >>= ob).noFailure ↔ oa.noFailure ∧ ∀ x ∈ oa.support, (ob x).noFailure := by
-  induction oa using OracleComp.inductionOn with
-  | pure x => simp
-  | failure => simp
-  | query_bind _ _ r ih =>
-    simp [ih]
-    constructor <;> intro h
-    · exact ⟨fun x => (h x).1, fun a x h' => (h x).2 a h'⟩
-    · exact fun x => ⟨h.1 x, fun a h' => h.2 a x h'⟩
+-- @[simp]
+-- lemma noFailure_bind_iff (oa : OracleComp spec α) (ob : α → OracleComp spec β) :
+--     (oa >>= ob).noFailure ↔ oa.noFailure ∧ ∀ x ∈ oa.support, (ob x).noFailure := by
+--   induction oa using OracleComp.inductionOn with
+--   | pure x => simp
+--   | failure => simp
+--   | query_bind _ _ r ih => simp [ih, forall_and]; tauto
 
-alias ⟨noFailure_bind, _⟩ := noFailure_bind_iff
+-- alias ⟨noFailure_bind, _⟩ := noFailure_bind_iff
 
-@[simp]
-lemma noFailure_map_iff (oa : OracleComp spec α) (f : α → β) :
-    noFailure (f <$> oa) ↔ noFailure oa := by
-  rw [map_eq_bind_pure_comp]
-  simp only [noFailure_bind_iff, Function.comp_apply, noFailure_pure, implies_true, and_true]
+-- @[simp]
+-- lemma noFailure_map_iff (oa : OracleComp spec α) (f : α → β) :
+--     noFailure (f <$> oa) ↔ noFailure oa := by
+--   rw [map_eq_bind_pure_comp]
+--   simp only [noFailure_bind_iff, Function.comp_apply, noFailure_pure, implies_true, and_true]
 
-@[simp]
-instance {α : Type u} [spec.FiniteRange] : DecidablePred (@OracleComp.noFailure _ spec α) :=
-  fun oa => by induction oa using OracleComp.construct with
-  | pure x =>
-      refine Decidable.isTrue (noFailure_pure x)
-  | failure =>
-      refine Decidable.isFalse not_noFailure_failure
-  | query_bind q _ r =>
-      cases q
-      simp only [noFailure_bind_iff, noFailure_query, support_liftM, Set.mem_univ, forall_const, true_and]
-      exact Fintype.decidableForallFintype
+-- @[simp]
+-- instance {α : Type u} [spec.FiniteRange] : DecidablePred (@OracleComp.noFailure _ spec α) :=
+--   fun oa => by induction oa using OracleComp.construct' with
+--   | pure x => exact Decidable.isTrue (noFailure_pure x)
+--   | failure => exact Decidable.isFalse not_noFailure_failure
+--   | query_bind i t _ r =>
+--       simpa only [noFailure_bind_iff, noFailure_query, support_liftM, Set.mem_univ,
+--         forall_const, true_and] using Fintype.decidableForallFintype
 
-section List
+-- section List
 
-open List
+-- open List
 
-/-- If each element of a list is mapped to a computation that never fails, then the computation
-  obtained by monadic mapping over the list also never fails. -/
-@[simp] lemma noFailure_list_mapM {f : α → OracleComp spec β} {as : List α}
-    (h : ∀ x ∈ as, noFailure (f x)) : noFailure (mapM f as) := by
-  induction as with
-  | nil => simp only [mapM, mapM.loop, reverse_nil, noFailure_pure]
-  | cons a as ih =>
-    simp [mapM_cons, h]
-    exact fun _ _ => ih (by simp at h; exact h.2)
+-- /-- If each element of a list is mapped to a computation that never fails, then the computation
+--   obtained by monadic mapping over the list also never fails. -/
+-- @[simp] lemma noFailure_list_mapM {f : α → OracleComp spec β} {as : List α}
+--     (h : ∀ x ∈ as, noFailure (f x)) : noFailure (mapM f as) := by
+--   induction as with
+--   | nil => simp only [mapM, mapM.loop, reverse_nil, noFailure_pure]
+--   | cons a as ih =>
+--     simp [mapM_cons, h]
+--     exact fun _ _ => ih (by simp at h; exact h.2)
 
-@[simp] lemma noFailure_list_mapM' {f : α → OracleComp spec β} {as : List α}
-    (h : ∀ x ∈ as, noFailure (f x)) : noFailure (mapM' f as) := by
-  rw [mapM'_eq_mapM]
-  exact noFailure_list_mapM h
+-- @[simp] lemma noFailure_list_mapM' {f : α → OracleComp spec β} {as : List α}
+--     (h : ∀ x ∈ as, noFailure (f x)) : noFailure (mapM' f as) := by
+--   rw [mapM'_eq_mapM]
+--   exact noFailure_list_mapM h
 
-@[simp] lemma noFailure_list_flatMapM {f : α → OracleComp spec (List β)} {as : List α}
-    (h : ∀ x ∈ as, noFailure (f x)) : noFailure (flatMapM f as) := by
-  induction as with
-  | nil => simp only [flatMapM_nil, noFailure_pure]
-  | cons a as ih =>
-    simp only [flatMapM_cons, bind_pure_comp, noFailure_bind_iff, noFailure_map_iff]
-    exact ⟨h a (by simp), fun y hy => ih (fun x hx => h x (by simp [hx]))⟩
+-- @[simp] lemma noFailure_list_flatMapM {f : α → OracleComp spec (List β)} {as : List α}
+--     (h : ∀ x ∈ as, noFailure (f x)) : noFailure (flatMapM f as) := by
+--   induction as with
+--   | nil => simp only [flatMapM_nil, noFailure_pure]
+--   | cons a as ih =>
+--     simp only [flatMapM_cons, bind_pure_comp, noFailure_bind_iff, noFailure_map_iff]
+--     exact ⟨h a (by simp), fun y hy => ih (fun x hx => h x (by simp [hx]))⟩
 
-@[simp] lemma noFailure_list_filterMapM {f : α → OracleComp spec (Option β)} {as : List α}
-    (h : ∀ x ∈ as, noFailure (f x)) : noFailure (filterMapM f as) := by
-  induction as with
-  | nil => simp only [filterMapM_nil, noFailure_pure]
-  | cons a as ih =>
-    simp only [filterMapM_cons, bind_pure_comp, noFailure_bind_iff, noFailure_map_iff]
-    refine ⟨h a (by simp), fun y hy => ?_⟩
-    rcases y with _ | y <;> simp <;> exact ih (fun x hx => h x (by simp [hx]))
+-- @[simp] lemma noFailure_list_filterMapM {f : α → OracleComp spec (Option β)} {as : List α}
+--     (h : ∀ x ∈ as, noFailure (f x)) : noFailure (filterMapM f as) := by
+--   induction as with
+--   | nil => simp only [filterMapM_nil, noFailure_pure]
+--   | cons a as ih =>
+--     simp only [filterMapM_cons, bind_pure_comp, noFailure_bind_iff, noFailure_map_iff]
+--     refine ⟨h a (by simp), fun y hy => ?_⟩
+--     rcases y with _ | y <;> simp <;> exact ih (fun x hx => h x (by simp [hx]))
 
-variable {s : Type v}
+-- variable {s : Type v}
 
-@[simp] lemma noFailure_list_foldlM {f : s → α → OracleComp spec s} {init : s} {as : List α}
-    (h : ∀ i, ∀ x ∈ as, noFailure (f i x)) : noFailure (foldlM f init as) := by
-  induction as generalizing init with
-  | nil => simp only [foldlM, reverse_nil, noFailure_pure]
-  | cons b bs ih =>
-      simp only [foldlM_cons, noFailure_bind_iff, mem_cons, true_or, h, true_and]
-      exact fun _ _ => ih (fun i x hx' => h i x (by simp [hx']))
+-- @[simp] lemma noFailure_list_foldlM {f : s → α → OracleComp spec s} {init : s} {as : List α}
+--     (h : ∀ i, ∀ x ∈ as, noFailure (f i x)) : noFailure (foldlM f init as) := by
+--   induction as generalizing init with
+--   | nil => simp only [foldlM, reverse_nil, noFailure_pure]
+--   | cons b bs ih =>
+--       simp only [foldlM_cons, noFailure_bind_iff, mem_cons, true_or, h, true_and]
+--       exact fun _ _ => ih (fun i x hx' => h i x (by simp [hx']))
 
-@[simp] lemma noFailure_list_foldrM {f : α → s → OracleComp spec s} {init : s} {as : List α}
-    (h : ∀ i, ∀ x ∈ as, noFailure (f x i)) : noFailure (foldrM f init as) := by
-  induction as generalizing init with
-  | nil => simp only [foldrM, reverse_nil, foldlM_nil, noFailure_pure]
-  | cons b bs ih =>
-      simp only [foldrM_cons, noFailure_bind_iff]
-      exact ⟨ih (fun i x hx => h i x (by simp [hx])), fun y _ => h y b (by simp)⟩
+-- @[simp] lemma noFailure_list_foldrM {f : α → s → OracleComp spec s} {init : s} {as : List α}
+--     (h : ∀ i, ∀ x ∈ as, noFailure (f x i)) : noFailure (foldrM f init as) := by
+--   induction as generalizing init with
+--   | nil => simp only [foldrM, reverse_nil, foldlM_nil, noFailure_pure]
+--   | cons b bs ih =>
+--       simp only [foldrM_cons, noFailure_bind_iff]
+--       exact ⟨ih (fun i x hx => h i x (by simp [hx])), fun y _ => h y b (by simp)⟩
 
--- TODO: add lemmas for more monadic list operations
+-- -- TODO: add lemmas for more monadic list operations
 
-end List
+-- end List
 
-section List.Vector
+-- section List.Vector
 
-variable {n : ℕ}
+-- variable {n : ℕ}
 
-@[simp] lemma noFailure_list_vector_mmap {f : α → OracleComp spec β} {as : List.Vector α n}
-    (h : ∀ x ∈ as.toList, noFailure (f x)) : noFailure (List.Vector.mmap f as) := by
-  induction as with
-  | nil => simp only [List.Vector.mmap, noFailure_pure]
-  | @cons n x xs ih =>
-    simp only [List.Vector.mmap_cons, bind_pure_comp, noFailure_bind_iff, noFailure_map_iff]
-    exact ⟨h x (by simp), fun y hy => ih (fun x' hx' => h x' (by simp [hx']))⟩
+-- @[simp] lemma noFailure_list_vector_mmap {f : α → OracleComp spec β} {as : List.Vector α n}
+--     (h : ∀ x ∈ as.toList, noFailure (f x)) : noFailure (List.Vector.mmap f as) := by
+--   induction as with
+--   | nil => simp only [List.Vector.mmap, noFailure_pure]
+--   | @cons n x xs ih =>
+--     simp only [List.Vector.mmap_cons, bind_pure_comp, noFailure_bind_iff, noFailure_map_iff]
+--     exact ⟨h x (by simp), fun y hy => ih (fun x' hx' => h x' (by simp [hx']))⟩
 
-end List.Vector
+-- end List.Vector
 
-section Array
+-- section Array
 
-open Array
+-- open Array
 
-@[simp] lemma noFailure_array_mapM {f : α → OracleComp spec β} {as : Array α}
-    (h : ∀ x ∈ as, noFailure (f x)) : noFailure (mapM f as) := by
-  induction ha : as.toList generalizing as with
-  | nil => simp_all [h, Array.mapM, mapM.map, noFailure_pure]
-  | cons x xs ih =>
-    simp_rw [mapM_eq_mapM_toList, ha] at ih ⊢
-    simp at ih ⊢
-    -- boring case analysis
-    sorry
+-- -- @[simp] lemma noFailure_array_mapM {f : α → OracleComp spec β} {as : Array α}
+-- --     (h : ∀ x ∈ as, noFailure (f x)) : noFailure (mapM f as) := by
+-- --   induction ha : as.toList generalizing as with
+-- --   | nil => simp_all [h, Array.mapM, mapM.map, noFailure_pure]
+-- --   | cons x xs ih =>
+-- --     rw [mapM_eq_mapM_toList, noFailure_map_iff]
 
-end Array
+-- --     simp_rw [mapM_eq_mapM_toList, ha] at ih ⊢
+-- --     simp at ih ⊢
+-- --     specialize ih h
+-- --     -- boring case analysis
+-- --     sorry
 
-section Vector
+-- end Array
 
-open Vector
+-- section Vector
 
-variable {n : ℕ}
+-- open Vector
 
--- Need induction principle for vectors
-@[simp] lemma noFailure_vector_mapM {f : α → OracleComp spec β} {xs : Vector α n}
-    (h : ∀ x ∈ xs.toList, noFailure (f x)) : noFailure (mapM f xs) := by sorry
-  -- match h : xs with
-  -- | ⟨⟨[]⟩, _⟩ => simp [Vector.mapM, Vector.mapM.go, noFailure_pure]
-  -- | ⟨⟨x :: xs⟩, _⟩ =>
-  --   simp only [mapM_cons, bind_pure_comp, noFailure_bind_iff, noFailure_map_iff]
-  --   exact ⟨h x (by simp), fun y hy => ih (fun x' hx' => h x' (by simp [hx']))⟩
+-- -- variable {n : ℕ}
 
-end Vector
+-- -- -- Need induction principle for vectors
+-- -- @[simp] lemma noFailure_vector_mapM {f : α → OracleComp spec β} {xs : Vector α n}
+-- --     (h : ∀ x ∈ xs.toList, noFailure (f x)) : noFailure (mapM f xs) := by sorry
+-- --   -- match h : xs with
+-- --   -- | ⟨⟨[]⟩, _⟩ => simp [Vector.mapM, Vector.mapM.go, noFailure_pure]
+-- --   -- | ⟨⟨x :: xs⟩, _⟩ =>
+-- --   --   simp only [mapM_cons, bind_pure_comp, noFailure_bind_iff, noFailure_map_iff]
+-- --   --   exact ⟨h x (by simp), fun y hy => ih (fun x' hx' => h x' (by simp [hx']))⟩
 
-end OracleComp
+-- end Vector
+
+-- end OracleComp
